demo/union_find/UnionFind1.v
@@ -1,0 +1,88 @@
+Require Import CoqlibC Maps.
+Require Import ASTC Integers ValuesC EventsC MemoryC Globalenvs.
+Require Import Op Registers.
+Require Import sflib.
+Require Import SmallstepC.
+Require Export Simulation.
+Require Import Skeleton Mod ModSem.
+Require ClightC.
+Require Import UnionFindHeader.
+Require Import UnionFind0.
+Require Import SIRStack.
+(* Require Import Clightdefs. *)
+
+Set Implicit Arguments.
+
+
+Let f_new_alt (oh0: owned_heap) (m0: mem) (vs0: list val):
+  itree (E owned_heap) (owned_heap * (mem * val)) :=
+  unwrapU (do _ <- parg_new vs0 ;
+           do (m1, b) <- malloc m0 (Ptrofs.repr 12) ;
+           let x  := Vptr b Ptrofs.zero in
+           do m2 <- Mem.store Mptr   m1 b 4 x ;
+           do m3 <- Mem.store Mint32 m2 b 0 (Vint Int.zero) ;
+           Some (oh0, (m3, x))) >>= ret
+.
+
+(*** I will prefer below definition because it is more canonical; we can control unwarpU/unwrapN ***)
+Definition f_new (oh0: owned_heap) (m0: mem) (vs0: list val):
+  itree (E owned_heap) (owned_heap * (mem * val)) :=
+  _ <- unwrapU (parg_new vs0) ;;
+  '(m1, b) <- unwrapU (malloc m0 (Ptrofs.repr 12)) ;;
+  let x  := Vptr b Ptrofs.zero in
+  m2 <- unwrapU (Mem.store Mptr m1 b 4 x) ;;
+  m3 <- unwrapU (Mem.store Mint32 m2 b 0 (Vint Int.zero)) ;;
+  Ret (oh0, (m3, x))
+.
+
+Goal f_new_alt = f_new.
+  apply func_ext3. ii. unfold f_new_alt, f_new.
+  irw. unfold unwrapU. unfold o_bind2, curry2. uo. unfold triggerUB.
+  repeat (des_ifs; ss; irw); try (by grind).
+Qed.
+
+Definition f_find (oh0: owned_heap) (m0: mem) (vs0: list val):
+  itree (E owned_heap) (owned_heap * (mem * val)) :=
+  x <- unwrapU (parg_find vs0) ;;
+  p <- unwrapU (Mem.load Mptr m0 x 4) ;;
+  cond <- unwrapU (Val.cmplu_bool (Mem.valid_pointer m0) Cne p (Vptr x Ptrofs.zero)) ;;
+  myif (cond)
+    ('(oh1, (m1, p0)) <- trigger (ICall _find oh0 m0 [p]) ;;
+      m2 <- unwrapU (Mem.store Mptr m1 x 4 p0) ;;
+      Ret (oh1, (m2, p0)))
+    (Ret (oh0, (m0, p)))
+.
+
+Definition f_union (oh0: owned_heap) (m0: mem) (vs0: list val):
+  itree (E owned_heap) (owned_heap * (mem * val)) :=
+  '(x, y) <- unwrapU (parg_union vs0) ;;
+  '(oh1, (m1, xRoot)) <- trigger (ICall _find oh0 m0 [Vptr x Ptrofs.zero]) ;;
+  '(oh2, (m2, yRoot)) <- trigger (ICall _find oh0 m0 [Vptr x Ptrofs.zero]) ;;
+  cond <- unwrapU (Val.cmplu_bool (Mem.valid_pointer m2) Ceq xRoot yRoot) ;;
+  (myif cond
+        (Ret (oh2, (m2, Vundef)))
+        (` xRootB: block <- unwrapU (unblock xRoot) ;;
+         ` yRootB: block <- unwrapU (unblock yRoot) ;;
+         xRank <- unwrapU (Mem.load Mint32 m2 xRootB 0) ;;
+         yRank <- unwrapU (Mem.load Mint32 m2 yRootB 0) ;;
+         myif (Val.cmp_bool Clt xRank yRank)
+              (m3 <- unwrapU (Mem.store Mptr m2 xRootB 4 yRoot) ;;
+               Ret (oh2, (m3, Vundef)))
+              (myif (Val.cmp_bool Cgt xRank yRank)
+                    (m3 <- unwrapU (Mem.store Mptr m2 yRootB 4 xRoot) ;;
+                     Ret (oh2, (m3, Vundef)))
+                    (m3 <- unwrapU (Mem.store Mptr m2 yRootB 4 xRoot) ;;
+                     m4 <- unwrapU (Mem.store Mint32 m3 xRootB 0 (Val.add xRank (Vint Int.one))) ;;
+                     Ret (oh2, (m4, Vundef)))
+              )
+        )
+  )
+.
+(*** TODO: Add notation for myif (proper align with automatic align) ***)
+
+
+(*** TODO: Add infix notation for Maps.add ***)
+Definition prog: program owned_heap :=
+  (Maps.add _union f_union (Maps.add _find f_find (Maps.add _new f_new Maps.empty))).
+
+Program Definition module: SMod.t _ := SMod.mk (UnionFind0.module) prog "fib"%string initial_owned_heap _.
