demo/union_find/UnionFindHeader.v
@@ -1,0 +1,69 @@
+Require Import CoqlibC Maps.
+Require Import ASTC Integers ValuesC EventsC MemoryC Globalenvs.
+Require Import Op Registers.
+Require Import sflib.
+Require Import SmallstepC.
+Require Export Simulation.
+Require Import Skeleton Mod ModSem.
+Require ClightC.
+Require Import UnionFind0.
+Require Import SIR.
+Require Export AuxBuffer.
+(* Require Import Clightdefs. *)
+
+Set Implicit Arguments.
+
+
+
+Definition owned_heap: Type := unit.
+Definition initial_owned_heap: SkEnv.t -> owned_heap := fun _ => tt.
+
+(*** TODO: move to CoqlibC ***)
+Coercion is_some_coercion {X}: (option X) -> bool := is_some.
+
+(*** TODO: move to more root ***)
+Global Opaque ident_eq.
+Global Opaque Z.of_nat.
+
+(*** TODO: move to better place ***)
+Definition unblock (v: val): option block :=
+  match v with
+  | Vptr x ofs =>
+    if Ptrofs.eq_dec ofs Ptrofs.zero
+    then Some x
+    else None
+  | _ => None
+  end
+.
+
+Definition malloc (m0: mem) (sz: ptrofs): option (mem * block) :=
+  let (m1, b) := Mem.alloc m0 (-8) (Ptrofs.unsigned sz) in
+  do m2 <- Mem.store Mptr m1 b (-8) (Vptrofs sz) ; Some (m2, b)
+.
+
+Definition parg_new (vs0: list val): option unit :=
+  match vs0 with
+  | [] => Some tt
+  | _ => None
+  end
+.
+
+Definition parg_find (vs0: list val): option block :=
+  match vs0 with
+  | [v] => unblock v
+  | _ => None
+  end
+.
+
+Definition parg_union (vs0: list val): option (block * block) :=
+  match vs0 with
+  | [x ; y] =>
+    match unblock x, unblock y with
+    | Some x, Some y => Some (x, y)
+    | _, _ => None
+    end
+  | _ => None
+  end
+.
+
+Global Obligation Tactic := sk_incl_tac.
